:PROPERTIES:
:ID:       c1c24a72-cdd2-4f19-a0f1-a4a2cb3d9258
:END:
#+title: Conjugate Gradient
#+filetags: :LinearAlgebra:
#+startup: latexpreview

Conjugate gradient is a method based on [[id:dc6424ca-a277-43f0-b37c-753435090ea2][Krylov subspace]] which aims at
minimizing the following quadratic function $\phi(x) = x^TAx - b^Tb$ for $A$ symmetric of size $n\times n$.
This is equivalent to solving the linear system $Ax = b$ for $x$.

At step $k$, the linear system residual is $r_k = Ax_k - b$
* Algorithm
  Let $x_0$, $r_0 = Ax_0 - b$, $p_0 = -r0$
  + While $\|r_k\|\neq 0$
    + The descent direction is $p_k$
    + The step size is $\alpha_k = \frac{r_k^Tr_k}{p_k^TAp_k} = \frac{\langle r_k, r_k \rangle}{\langle p_k, Ap_k \rangle}$
    + The new iterate $x_{k+1} = x_k + \alpha_k p_k$
    + The new residual $r_{k+1} = Ax_{k+1} = Ax_k + \alpha_k A p_k = r_k + \alpha_k A p_k$
    + $\beta_{k+1} = \frac{r_{k+1}^Tr_{k+1}}{r_k^Tr_k} = \frac{\|r_{k+1}\|^2}{\|r_k\|^2}$
    + The new descent direction is $p_{k+1} = -r_{k+1} + \beta_{k+1} p_k$
    + $k \gets k+1$
      
* Explanation
  Let us say we have a set of orthogonal directions $p_k$.
  We start from the fact that we want an iteration of the form $x_{k+1} = x_k + \alpha_k p_k$
  We want the residual to be orthogonal to the current descent direction, so $r_k^Tp_k = 0$
  \begin{align}
p_k^Tr_{k+1} &= p_k^T\left(Ax_{k+1} - b \right) \\
             &= p_k^T(r_k + \alpha_kAp_k) \\
             &= p_k^Tr_k + \alpha_k p_k^TAp_k = 0 \\
\alpha_k &= - \frac{p_k^Tr_k}{p_k^TAp_k}
  \end{align}


* Convergence rate

Using Conjugate Gradient, the error $e_k = x_k - x^*$ can be bounded:
\begin{align}
    \|e_k\| &\leq 2\left(\frac{\sqrt{\kappa(A)} - 1}{\sqrt{\kappa(A)} + 1}\right)^k \|e_0\| 
   % \\ \log \|e_k\| &\leq \log 2 + \log \| e_0 \| + k \log \left(\frac{\sqrt{\kappa(A)}-1}{\sqrt{\kappa(A)}+1}\right)
\end{align}
where $\kappa$ is the [[id:4a033759-84da-4099-b6dc-1df50308f966][Condition number]] of $A$.
We have the following asymptotic equivalent:
\begin{equation}
\frac{\sqrt{\kappa(A)} - 1}{\sqrt{\kappa(A)} + 1} = 1 -  \frac{2}{\sqrt{\kappa}} + \mathcal{O}(\kappa^{-1})
\end{equation}
